thys/Word_Lib/Word_16.thy
@@ -1,0 +1,18 @@
+(*
+ * Copyright 2020, Data61, CSIRO (ABN 41 687 119 230)
+ *
+ * SPDX-License-Identifier: BSD-2-Clause
+ *)
+
+section "Words of Length 16"
+
+theory Word_16
+imports
+  Word_Lemmas
+  Word_Syntax
+begin
+
+type_synonym word16 = "16 word"
+lemma len16: "len_of (x :: 16 itself) = 16" by simp
+
+end
