thys/Word_Lib/Word_8.thy
@@ -1,0 +1,18 @@
+(*
+ * Copyright 2020, Data61, CSIRO (ABN 41 687 119 230)
+ *
+ * SPDX-License-Identifier: BSD-2-Clause
+ *)
+
+section "Words of Length 8"
+
+theory Word_8
+imports
+  Word_Lemmas
+  Word_Syntax
+begin
+
+type_synonym word8 = "8 word"
+lemma len8: "len_of (x :: 8 itself) = 8" by simp
+
+end
