thys/Word_Lib/Word_Syntax.thy
@@ -9,20 +9,9 @@ section "Additional Syntax for Word Bit Operations"
 theory Word_Syntax
 imports
   "HOL-Library.Word"
-  Bitwise
 begin
 
 text \<open>Additional bit and type syntax that forces word types.\<close>
-
-type_synonym word8 = "8 word"
-type_synonym word16 = "16 word"
-type_synonym word32 = "32 word"
-type_synonym word64 = "64 word"
-
-lemma len8: "len_of (x :: 8 itself) = 8" by simp
-lemma len16: "len_of (x :: 16 itself) = 16" by simp
-lemma len32: "len_of (x :: 32 itself) = 32" by simp
-lemma len64: "len_of (x :: 64 itself) = 64" by simp
 
 abbreviation
   wordNOT  :: "'a::len word \<Rightarrow> 'a word"      ("~~ _" [70] 71)
